passed through RunsToRelax.v. Proving in CompileStatement.v

platform/cito/RunsToRelax.v
@@ -1,8 +1,104 @@
 Require Import SyntaxExpr SemanticsExpr.
 Require Import Syntax Semantics SyntaxNotations.
 Require Import VariableLemmas.
-Require Import Depth.
+Require Import Depth Footprint.
 Require Import GeneralTactics.
+Require Import ExprLemmas.
+Require Import SemanticsLemmas.
+Require Import Arith.
+
+Open Scope nat.
+
+Lemma le_max_l_trans : forall a b c, (a <= b -> a <= max b c)%nat.
+  intros; eapply le_trans.
+  2: eapply Max.le_max_l.
+  eauto.
+Qed.
+
+Lemma le_max_r_trans : forall a b c, (a <= c -> a <= max b c)%nat.
+  intros; eapply le_trans.
+  2: eapply Max.le_max_r.
+  eauto.
+Qed.
+
+Ltac max_le_solver :=
+  repeat 
+    match goal with
+      | |- ?A <= ?A => eapply le_n
+      | |- max ?A ?B <= _ => eapply Max.max_lub
+      | |- ?S <= max ?A _ =>
+        match A with
+          context [ S ] => eapply le_max_l_trans
+        end
+      | |- ?S <= max _ ?B =>
+        match B with
+          context [ S ] => eapply le_max_r_trans
+        end
+    end.
+
+Ltac incl_app_solver :=
+  repeat 
+    match goal with
+      | |- List.incl ?A ?A => eapply List.incl_refl
+      | |- List.incl (?A ++ ?B) _ => eapply incl_app
+      | |- List.incl (?A :: ?B) _ => eapply List.incl_cons
+      | |- List.incl ?S (?A ++ _) =>
+        match A with
+          context [ S ] => eapply incl_appl
+        end
+      | |- List.incl ?S (_ ++ ?B) =>
+        match B with
+          context [ S ] => eapply incl_appr
+        end
+      | |- List.incl ?S (?A :: _) =>
+        match A with
+          context [ S ] => eapply (@incl_appl _ _ _ (_ :: nil))
+        end
+      | |- List.incl ?S (?A :: ?B) =>
+        match B with
+          context [ S ] => eapply (@incl_appr _ _ (_ :: nil))
+        end
+    end.
+
+Ltac change_RunsTo_for_goal :=
+  match goal with
+    H : RunsTo _ ?S ?VS1 _ |- context [ RunsTo _ ?S ?VS1' _ ] => generalize H; eapply RunsTo_immune with (vs1' := VS1') in H; intros
+  end.
+
+Ltac apply_in_all t :=
+  repeat match goal with
+           H : _ |- _ => eapply t in H
+         end.
+
+Ltac use_changed_in_eval :=
+  match goal with
+    H : VariableLemmas.equiv ?V (merge _ _ _) |- changed_in ?V _ _ =>
+      apply_in_all RunsTo_footprint; eapply changed_in_eval; [eassumption | ..]
+  end.
+
+Ltac auto_apply_in t :=
+  match goal with
+    H : _ |- _ => eapply t in H
+  end.
+
+Ltac use_disjoint_trans'' := 
+  match goal with
+    | H : disjoint ?A ?B |- disjoint ?C _ =>
+      match A with context [ C ] =>
+        eapply (@disjoint_trans_lr _ A B C _ H)
+      end 
+    | H : disjoint ?A ?B |- disjoint (?C1 ++ ?C2) _ =>
+      match A with context [ C1 ] =>
+        match A with context [ C2 ] =>
+          eapply (@disjoint_trans_lr _ A B (C1 ++ C2) _ H)
+        end
+      end 
+  end.
+
+Ltac change_RunsTo_to t :=
+  match goal with
+    H : RunsTo _ ?S ?VS1 _ |- _ => generalize H; eapply RunsTo_immune with (vs1' := t) in H; intros
+  end.
 
 Section Hints.
 
@@ -12,9 +108,68 @@ Section Hints.
       /\ snd v_new = snd v'.
 
   Local Notation "fs ~:~ v1 ~~ s ~~> v2" := (RunsToRelax fs s v1 v2) (no associativity, at level 60).
-
   Local Notation "v [( e )]" := (exprDenote e (fst v)) (no associativity, at level 60).
-  
+  Local Notation agree_except := changed_in.
+  Local Notation "'tmps' s" := (tempVars (depth s)) (at level 60).
+  Local Notation edepth := DepthExpr.depth.
+  Local Notation "'etmps' s" := (tempVars (edepth s)) (at level 60).
+  Local Notation "v [ e ]" := (exprDenote e v) (no associativity, at level 60).
+  Local Notation "b [ vars => c ]" := (merge c b vars) (no associativity, at level 60).
+  Local Notation agree_except_trans := changedVariables_trans.
+  Local Notation "fs -:- v1 -- s --> v2" := (RunsTo fs s v1 v2) (no associativity, at level 60).
+  Infix "==" := VariableLemmas.equiv.
+
+  Definition st_agree_except (v1 v2 : st) vars := agree_except (fst v1) (fst v2) vars /\ snd v1 = snd v2.
+
+  Local Notation "v1 =~= v2 [^ except ]" := (st_agree_except v1 v2 except) (no associativity, at level 60).
+
+  Hint Rewrite sum_S : arith.
+  Hint Resolve S_le_lt.
+  Hint Resolve sel_upd_firstn.
+  Hint Resolve firstn_S_upd.
+  Hint Resolve VariableLemmas.noChange.
+  Hint Resolve Max.le_max_l Max.le_max_r.
+  Hint Extern 12 => rv_solver.
+  Hint Extern 12 => sp_solver.
+  Hint Resolve le_plus_lt lt_max_l lt_max_r.
+  Hint Resolve plus_le.
+  Hint Resolve lt_le_S plus_lt.
+
+  Hint Resolve le_max_l_trans.
+  Hint Resolve le_max_r_trans.
+  Hint Extern 0 (_ <= _) => progress max_le_solver.
+  Hint Extern 0 (List.incl _ _) => progress incl_app_solver.
+
+  Hint Resolve in_eq In_incl.
+  Hint Resolve List.incl_cons incl_cons_l incl_cons_r List.incl_refl incl_nil incl_tl incl_array.
+  Hint Resolve incl_app incl_appl incl_appr.
+  Hint Resolve List.incl_tran.
+  Hint Resolve disjoint_trans_lr.
+  Hint Resolve changedVariables_upd.
+  Hint Resolve unchanged_in_except_disjoint unchanged_in_except_upd unchanged_in_except_shrink.
+  Hint Constructors or.
+  Hint Resolve sel_upd_eq.
+
+  Hint Constructors RunsTo.
+  Hint Constructors runs_loop_partially.
+  Hint Resolve unchanged_exprDenote.
+  Hint Resolve changedVariables_upd_bwd.
+  Hint Resolve unchanged_incl.
+  Hint Resolve two_merge_equiv.
+  Hint Resolve changed_in_upd_same.
+
+  Hint Extern 12 (unchanged_in _ _ _) => use_changed_unchanged.
+  Hint Extern 12 (unchanged_in _ _ _) => use_changed_unchanged'.
+  Hint Extern 12 (changed_in _ _ _) => use_changed_trans2.
+  Hint Extern 12 (changed_in _ _ _) => use_changed_incl.
+  Hint Extern 12 => condition_solver'.
+  Hint Extern 12 (unchanged_in _ _ _) => use_unchanged_in_symm.
+  Hint Extern 12 (changed_in _ _ _) => use_changed_in_symm.
+
+  Hint Resolve runs_loop_partially_finish.
+  Hint Resolve exprDenote_disjoint.
+  Hint Resolve RunsTo_footprint.
+
   Lemma RunsToRelax_loop_false : forall fs e b k v1 v2, 
     fs ~:~ v1 ~~ k ~~> v2 -> 
     wneb (v1[(e)]) $0 = false -> 
@@ -23,6 +178,10 @@ Section Hints.
   Qed.
 
   Hint Resolve RunsToRelax_loop_false.
+
+  Lemma st_agree_except_symm : forall v1 v2 ex, v1 =~= v2 [^ex] -> v2 =~= v1 [^ex].
+    unfold st_agree_except; intuition.
+  Qed.
 
   Lemma RunsToRelax_immune : forall fs s v1 v2 v1' v2', 
     fs ~:~ v1 ~~ s ~~> v2 ->
@@ -34,6 +193,10 @@ Section Hints.
     eauto.
     use_changed_in_eval; eauto; eapply changedVariables_symm in H0; eauto.
     congruence.
+  Qed.
+
+  Lemma inversion_RunsTo_seq : forall fs a b v1 v2, fs -:- v1 -- a;: b --> v2 -> exists v, fs -:- v1 -- a --> v /\ fs -:- v -- b --> v2.
+    inversion 1; eauto.
   Qed.
 
   Lemma RunsToRelax_cond_true' : forall fs e t f k v1 v2,
@@ -76,16 +239,63 @@ Section Hints.
 (*    intros; eapply RunsToRelax_immune; unfold s, st_agree_except in *; openhyp; descend; simpl in *; eauto.*)
   Qed.
 
-  Lemma RunsToRelax_assign : forall fs var e k v1 v2 v3,
-    fs ~:~ v2 ~~ k ~~> v3 ->
-    denote_sem (var <- e) v1 =~= v2 [^etmps e] ->
-    disjoint (footprint k) (etmps e) ->
-    fs ~:~ v1 ~~ var <- e;: k ~~> v3.
-    intros; eapply st_agree_except_symm in H0; unfold denote_sem, RunsToRelax, st_agree_except in *; openhyp; change_RunsTo_to (denote_sem (var <- e) v1); eauto; openhyp; destruct v1; simpl in *; descend.
+  Lemma changed_trans_l : forall vs1 vs2 vs3 a c, 
+    changedVariables vs1 vs2 a -> 
+    changedVariables vs2 vs3 c ->
+    List.incl a c ->
+    changedVariables vs1 vs3 c.
     eauto.
-    eapply changedVariables_symm in H0; use_changed_in_eval; eauto.
-    congruence.
   Qed.
+
+  Definition tmps_diff big small := tempChunk (depth small) (depth big - depth small).
+
+  Lemma incl_tempChunk2 : forall b n m, b + n <= m -> List.incl (tempChunk b n) (tempVars m).
+    intros; eapply incl_tempChunk; eauto.
+  Qed.
+
+  Hint Resolve incl_tempChunk2.
+
+  Lemma agree_except_app_comm : forall vs1 vs2 a b,
+    agree_except vs1 vs2 (a ++ b) ->
+    agree_except vs1 vs2 (b ++ a).
+    intros; eauto.
+  Qed.
+
+  Lemma merge_comm : forall v vars1 v1 vars2 v2,
+    disjoint vars1 vars2 ->
+    v [vars1 => v1] [vars2 => v2] == v [vars2 => v2] [vars1 => v1].
+    intros.
+    unfold VariableLemmas.equiv, changedVariables.
+    intros.
+    contradict H0.
+    destruct (In_dec string_dec x vars1).
+    destruct (In_dec string_dec x vars2).
+    unfold disj in *.
+    contradict H.
+    eauto.
+    rewrite sel_merge by eauto.
+    rewrite sel_merge_outside by eauto.
+    rewrite sel_merge by eauto.
+    eauto.
+    destruct (In_dec string_dec x vars2).
+    rewrite sel_merge_outside by eauto.
+    rewrite sel_merge by eauto.
+    rewrite sel_merge by eauto.
+    eauto.
+    rewrite sel_merge_outside by eauto.
+    rewrite sel_merge_outside by eauto.
+    rewrite sel_merge_outside by eauto.
+    rewrite sel_merge_outside by eauto.
+    eauto.
+  Qed.
+
+  Lemma equiv_merge_equiv : forall v1 v2 vars v,
+    v1 == v2 ->
+    v1 [vars => v] == v2 [vars => v].
+    intros; eapply two_merge_equiv; eauto.
+  Qed.
+
+  Hint Extern 1 => use_disjoint_trans''.
 
   Lemma RunsToRelax_seq_fwd : forall fs a b v1 v2,
     fs ~:~ v1 ~~ a;: b ~~> v2 ->
@@ -183,6 +393,15 @@ Section Hints.
     clear; simpl; intros; eapply RunsToRelax_seq_fwd in H; eauto; openhyp; eapply RunsToRelax_seq_fwd in H1; eauto; openhyp; repeat eapply RunsToRelax_seq_bwd; repeat (simpl; eauto).
   Qed.
 
+  Lemma RunsTo_loop_true : forall fs e b v1 v2,
+    fs -:- v1 -- b;: While e b --> v2 ->
+    wneb (v1[(e)]) $0 = true ->
+    fs -:- v1 -- While e b --> v2.
+    clear; intros; eapply inversion_RunsTo_seq in H; openhyp; eauto.
+  Qed.
+
+  Hint Resolve RunsTo_loop_true.
+
   Lemma RunsToRelax_loop_true : forall fs e b v1 v2, 
     fs ~:~ v1 ~~ b;: While e b ~~> v2 -> 
     wneb (v1[(e)]) $0 = true -> 
@@ -202,8 +421,6 @@ Section Hints.
   Qed.
 
   Hint Resolve RunsToRelax_loop_true_k.
-
-  Hint Resolve Safe_assoc_left.
 
   Lemma RunsToRelax_skip : forall fs s v1 v2,
     fs ~:~ v1 ~~ s ~~> v2 ->
