platform/cito/Syntax.v
@@ -6,5 +6,4 @@ Inductive Statement : Set :=
   | Seq : Statement -> Statement -> Statement
   | If : Expr -> Statement -> Statement -> Statement
   | While : Expr -> Statement -> Statement
-  | Assign : string -> Expr -> Statement
   | Call : option string -> Expr -> list Expr -> Statement.
