platform/cito/SyntaxNotations.v
@@ -1,8 +1,6 @@
 Require Import Syntax.
 
-Local Notation skip := Syntax.Skip.
+Notation skip := Syntax.Skip.
 
 Infix ";:" := Syntax.Seq (left associativity, at level 110).
-
-Infix "<-" := Syntax.Assign (at level 90, no associativity).
 
